started making state type abstract

Given_Clause_Loops/Prover_Lazy_List_Queue.thy
@@ -17,74 +17,81 @@ subsection \<open>Locales\<close>
 
 locale prover_lazy_list_queue =
   fixes
+    nil :: 's and
+    llist :: "'s \<Rightarrow> 'e llist" and
     empty :: 'q and
-    add_llist :: "'e llist \<Rightarrow> 'q \<Rightarrow> 'q" and
-    remove_llist :: "'e llist \<Rightarrow> 'q \<Rightarrow> 'q" and
+    add_stream :: "'s \<Rightarrow> 'q \<Rightarrow> 'q" and
+    remove_stream :: "'s \<Rightarrow> 'q \<Rightarrow> 'q" and
     pick_elem :: "'q \<Rightarrow> 'e \<times> 'q" and
-    llists :: "'q \<Rightarrow> 'e llist multiset"
+    streams :: "'q \<Rightarrow> 's multiset"
   assumes
-    llists_empty[simp]: "llists empty = {#}" and
-    llists_not_empty: "Q \<noteq> empty \<Longrightarrow> llists Q \<noteq> {#}" and
-    llists_add[simp]: "llists (add_llist es Q) = llists Q + {#es#}" and
-    llist_remove[simp]: "llists (remove_llist es Q) = llists Q - {#es#}" and
-    llists_pick_elem: "(\<exists>es \<in># llists Q. es \<noteq> LNil) \<Longrightarrow>
-      \<exists>e es. LCons e es \<in># llists Q \<and> fst (pick_elem Q) = e
-        \<and> llists (snd (pick_elem Q)) = llists Q - {#LCons e es#} + {#es#}"
+    llist_nil[simp]: "llist nil = LNil" and
+    streams_empty[simp]: "streams empty = {#}" and
+    streams_not_empty: "Q \<noteq> empty \<Longrightarrow> streams Q \<noteq> {#}" and
+    streams_add[simp]: "streams (add_stream es Q) = streams Q + {#es#}" and
+    streams_remove[simp]: "streams (remove_stream es Q) = streams Q - {#es#}" and
+    streams_pick_elem: "(\<exists>s \<in># streams Q. llist s \<noteq> LNil) \<Longrightarrow>
+      \<exists>s \<in># streams Q. \<exists>s'. llist s \<noteq> LNil \<and> llist s' = ltl (llist s)
+        \<and> fst (pick_elem Q) = lhd (llist s)
+        \<and> streams (snd (pick_elem Q)) = streams Q - {#s#} + {#s'#}"
 begin
 
 abbreviation has_elem :: "'q \<Rightarrow> bool" where
-  "has_elem Q \<equiv> \<exists>es \<in># llists Q. es \<noteq> LNil"
+  "has_elem Q \<equiv> \<exists>s \<in># streams Q. llist s \<noteq> LNil"
 
 inductive lqueue_step :: "'q \<times> 'e set \<Rightarrow> 'q \<times> 'e set \<Rightarrow> bool" where
-  lqueue_step_fold_add_llistI:
-  "lqueue_step (Q, D) (fold add_llist ess Q, D - \<Union> {lset es |es. es \<in> set ess})"
-| lqueue_step_fold_remove_llistI:
-  "lqueue_step (Q, D) (fold remove_llist ess Q, D \<union> \<Union> {lset es |es. es \<in> set ess})"
+  lqueue_step_fold_add_streamI:
+  "lqueue_step (Q, D) (fold add_stream ss Q, D - \<Union> {lset (llist s) |s. s \<in> set ss})"
+| lqueue_step_fold_remove_streamI:
+  "lqueue_step (Q, D) (fold remove_stream ss Q, D \<union> \<Union> {lset (llist s) |s. s \<in> set ss})"
 | lqueue_step_pick_elemI: "has_elem Q \<Longrightarrow>
   lqueue_step (Q, D) (snd (pick_elem Q), D \<union> {fst (pick_elem Q)})"
 
 lemma lqueue_step_idleI: "lqueue_step QD QD"
-  using lqueue_step_fold_add_llistI[of "fst QD" "snd QD" "[]", simplified] .
+  using lqueue_step_fold_add_streamI[of "fst QD" "snd QD" "[]", simplified] .
 
-lemma lqueue_step_add_llistI: "lqueue_step (Q, D) (add_llist es Q, D - lset es)"
-  using lqueue_step_fold_add_llistI[of _ _ "[es]", simplified] .
+lemma lqueue_step_add_streamI: "lqueue_step (Q, D) (add_stream s Q, D - lset (llist s))"
+  using lqueue_step_fold_add_streamI[of _ _ "[s]", simplified] .
 
-lemma lqueue_step_remove_llistI: "lqueue_step (Q, D) (remove_llist es Q, D \<union> lset es)"
-  using lqueue_step_fold_remove_llistI[of _ _ "[es]", simplified] .
+lemma lqueue_step_remove_streamI: "lqueue_step (Q, D) (remove_stream s Q, D \<union> lset (llist s))"
+  using lqueue_step_fold_remove_streamI[of _ _ "[s]", simplified] .
 
-lemma llists_fold_add_llist[simp]: "llists (fold add_llist es Q) = mset es + llists Q"
-  by (induct es arbitrary: Q) auto
+lemma streams_fold_add_stream[simp]: "streams (fold add_stream ss Q) = mset ss + streams Q"
+  by (induct ss arbitrary: Q) auto
 
-lemma llists_fold_remove_llist[simp]: "llists (fold remove_llist es Q) = llists Q - mset es"
-  by (induct es arbitrary: Q) auto
+lemma streams_fold_remove_stream[simp]: "streams (fold remove_stream ss Q) = streams Q - mset ss"
+  by (induct ss arbitrary: Q) auto
 
-inductive pick_lqueue_step_w_details :: "'q \<times> 'e set \<Rightarrow> 'e \<Rightarrow> 'e llist \<Rightarrow> 'q \<times> 'e set \<Rightarrow> bool" where
-  pick_lqueue_step_w_detailsI: "LCons e es \<in># llists Q \<Longrightarrow> fst (pick_elem Q) = e \<Longrightarrow>
-    llists (snd (pick_elem Q)) = llists Q - {#LCons e es#} + {#es#} \<Longrightarrow>
-    pick_lqueue_step_w_details (Q, D) e es (snd (pick_elem Q), D \<union> {e})"
+inductive
+  pick_lqueue_step_w_details :: "'q \<times> 'e set \<Rightarrow> 'e \<Rightarrow> 'e llist \<Rightarrow> 's \<Rightarrow> 's \<Rightarrow> 'q \<times> 'e set \<Rightarrow> bool"
+where
+  pick_lqueue_step_w_detailsI: "s \<in># streams Q \<Longrightarrow> llist s \<noteq> LNil \<Longrightarrow> llist s' = ltl (llist s) \<Longrightarrow>
+    fst (pick_elem Q) = lhd (llist s) \<Longrightarrow>
+    streams (snd (pick_elem Q)) = streams Q - {#s#} + {#s'#} \<Longrightarrow>
+    pick_lqueue_step_w_details (Q, D) e es s s' (snd (pick_elem Q), D \<union> {e})"
 
 inductive pick_lqueue_step :: "'q \<times> 'e set \<Rightarrow> 'q \<times> 'e set \<Rightarrow> bool" where
-  pick_lqueue_stepI: "pick_lqueue_step_w_details QD e es QD' \<Longrightarrow> pick_lqueue_step QD QD'"
+  pick_lqueue_stepI: "pick_lqueue_step_w_details QD e es s s' QD' \<Longrightarrow> pick_lqueue_step QD QD'"
 
 inductive
   remove_lqueue_step_w_details :: "'q \<times> 'e set \<Rightarrow> 'e llist list \<Rightarrow> 'q \<times> 'e set \<Rightarrow> bool"
 where
   remove_lqueue_step_w_detailsI:
-    "remove_lqueue_step_w_details (Q, D) ess
-       (fold remove_llist ess Q, D \<union> \<Union> {lset es |es. es \<in> set ess})"
+    "remove_lqueue_step_w_details (Q, D) ss
+       (fold remove_stream ss Q, D \<union> \<Union> {lset (llist s) |s. s \<in> set ss})"
 
 end
 
 locale fair_prover_lazy_list_queue =
-  prover_lazy_list_queue empty add_llist remove_llist pick_elem llists
+  prover_lazy_list_queue empty add_stream remove_stream pick_elem streams
   for
     empty :: 'q and
-    add_llist :: "'e llist \<Rightarrow> 'q \<Rightarrow> 'q" and
-    remove_llist :: "'e llist \<Rightarrow> 'q \<Rightarrow> 'q" and
+    add_stream :: "'e llist \<Rightarrow> 'q \<Rightarrow> 'q" and
+    remove_stream :: "'e llist \<Rightarrow> 'q \<Rightarrow> 'q" and
     pick_elem :: "'q \<Rightarrow> 'e \<times> 'q" and
-    llists :: "'q \<Rightarrow> 'e llist multiset" +
+    streams :: "'q \<Rightarrow> 'e llist multiset" +
   assumes fair: "chain lqueue_step QDs \<Longrightarrow> infinitely_often pick_lqueue_step QDs \<Longrightarrow>
-    LCons e es \<in># llists (fst (lnth QDs i)) \<Longrightarrow>
+    LCons e es \<in># streams (fst (lnth QDs i)) \<Longrightarrow>
     \<exists>j \<ge> i. (\<exists>ess. LCons e es \<in> set ess
         \<and> remove_lqueue_step_w_details (lnth QDs j) ess (lnth QDs (Suc j)))
       \<or> pick_lqueue_step_w_details (lnth QDs j) e es (lnth QDs (Suc j))"
@@ -94,7 +101,7 @@ lemma fair_strong:
   assumes
     chain: "chain lqueue_step QDs" and
     inf: "infinitely_often pick_lqueue_step QDs" and
-    es_in: "es \<in># llists (fst (lnth QDs i))" and
+    es_in: "es \<in># streams (fst (lnth QDs i))" and
     k_lt: "enat k < llength es"
   shows "\<exists>j \<ge> i.
     (\<exists>k' \<le> k. \<exists>ess. ldrop k' es \<in> set ess
@@ -104,7 +111,7 @@ lemma fair_strong:
 proof (induct k)
   case 0
   note zero_lt = this
-  have es_in': "LCons (lnth es 0) (ldrop (Suc 0) es) \<in># llists (fst (lnth QDs i))"
+  have es_in': "LCons (lnth es 0) (ldrop (Suc 0) es) \<in># streams (fst (lnth QDs i))"
     using es_in by (metis zero_lt ldrop_0 ldrop_enat ldropn_Suc_conv_ldropn zero_enat_def)
   show ?case
     using fair[OF chain inf es_in']
@@ -135,7 +142,7 @@ next
     assume "pick_lqueue_step_w_details (lnth QDs j) (lnth es k) (ldrop (enat (Suc k)) es)
       (lnth QDs (Suc j))"
     hence cons_in: "LCons (lnth es (Suc k)) (ldrop (enat (Suc (Suc k))) es)
-      \<in># llists (fst (lnth QDs (Suc j)))"
+      \<in># streams (fst (lnth QDs (Suc j)))"
       unfolding pick_lqueue_step_w_details.simps using sk_lt
       by (metis fst_conv ldrop_enat ldropn_Suc_conv_ldropn union_mset_add_mset_right
           union_single_eq_member)
